1D flux-tube

\begin{eqnarray}
\frac{\partial n_i}{\partial t} &=& 
-\nabla\cdot\left(n_i\mathbf{b}v_{i\|}\right) \\ \frac{\partial p_i}{\partial 
t} &=& -\nabla\cdot\left(p_i\mathbf{b}v_{i\|}\right) - 
\frac{2}{3}p_i\nabla\cdot\left(\mathbf{b}v_{i\|}\right) \\ 
\frac{\partial}{\partial t}\left(n_iv_{i\|}\right) &=& 
-\nabla\cdot\left(n_iv_{i\|} \mathbf{b}v_{i\|}\right) - {\bf b}\cdot{\nabla}p_i + E 
\end{eqnarray}
\begin{eqnarray}
n_e &=& n_i \\ \frac{\partial p_e}{\partial t} &=& 
-\nabla\cdot\left(p_e\mathbf{b}v_{e\|}\right) - 
\frac{2}{3}p_e\nabla\cdot\left(\mathbf{b}v_{e\|}\right)
\end{eqnarray}
\begin{eqnarray}
E &=& -{\bf b}\cdot{\nabla}p_e \\ v_{e\|} &=& v_{i\|}
\end{eqnarray}

(1D Scrape-off Layer (SOL))

2D drift-plane


\begin{eqnarray}
\frac{\partial n_e}{\partial t} &=& - \nabla\cdot\left(n_e\mathbf{v}_{E\times 
B}\right) + \nabla\cdot{\frac{1}{e}\mathbf{j}_{sh}}
\end{eqnarray}
\begin{eqnarray}
p_e &=& e n_e T_e
\end{eqnarray}
\begin{eqnarray}
\mathbf{v}_{E\timesB} = {\bf b} \times \nabla \Phi / B
\end{eqnarray}

with fixed $T_e$

\begin{eqnarray}
\frac{\partial \omega}{\partial t} &=& - 
\nabla\cdot\left(\omega\mathbf{v}_{E\times B}\right) + 
\nabla\left(p_e\nabla\times\frac{\mathbf{b}}{B}\right) + 
\nabla\cdot\mathbf{j}_{sh} \\ 
\nabla\cdot\left(\frac{1}{B^2}\nabla_\perp\Phi\right) &=& \omega
\end{eqnarray}
\begin{eqnarray}
\nabla\cdot{\mathbf{j}_{sh}} &=& \frac{n_e\Phi}{L_{\|}}
\end{eqnarray}

Blob2D-Te-Ti

\begin{eqnarray}
\frac{\partial n_e}{\partial t} &=& - \nabla\cdot\left(n_e\mathbf{v}_{E\times 
B}\right) + \nabla\cdot{\frac{1}{e}\mathbf{j}_{sh}} \\ \frac{\partial 
p_e}{\partial t} &=& - \nabla\cdot\left(p_e\mathbf{v}_{E\times B}\right) - 
\gamma_e p_e c_s \\ n_{h+} &=& n_e \\ \frac{\partial p_{h+}}{\partial t} &=& - 
\nabla\cdot\left(p_{h+}\mathbf{v}_{E\times B}\right) \\ \frac{\partial 
\omega}{\partial t} &=& - \nabla\cdot\left(\omega\mathbf{v}_{E\times B}\right) 
+ \nabla\left[\left(p_e + p_{h+}\right)\nabla\times\frac{\mathbf{b}}{B}\right] 
+ \nabla\cdot\mathbf{j}_{sh} \\ 
\nabla\cdot\left[\frac{1}{B^2}\nabla_\perp\left(\Phi + p_{h+}\right)\right] &=& 
\omega \\ \nabla\cdot{\mathbf{j}_{sh}} &=& \frac{n_e\Phi}{L_{\|}}
\end{eqnarray}

2D-drift-plane-turbulence-te-ti

\begin{eqnarray}
p_\mathrm{total} &=& \sum_a n_a T_a \\ \rho_\mathrm{total} &=& \sum_a A_a n_a \\
c_s &=& \sqrt{\frac{p_\mathrm{total}}{\rho_\mathrm{total}}} \\ 
\frac{\partial n_e}{\partial t} &=& - \nabla\cdot\left(n_e\mathbf{v}_{E\times 
B}\right) + \nabla\cdot{\frac{1}{e}\mathbf{j}_{sh}} + n_e c_s + S_n \\ 
\frac{\partial p_e}{\partial t} &=& - \nabla\cdot\left(p_e\mathbf{v}_{E\times 
B}\right) - \gamma_e p_e c_s + S_{p_e} \\
n_{h+} &=& n_e \\
\frac{\partial p_{h+}}{\partial t} &=& - \nabla\cdot\left(p_{h+}\mathbf{v}_{E\times B}\right) 
- \gamma_i p_{h+} c_s \\
\frac{\partial \omega}{\partial t} &=& 
-\nabla\cdot\left(\omega\mathbf{v}_{E\times B}\right) + \nabla\left[\left(p_e + 
p_{h+}\right)\nabla\times\frac{\mathbf{b}}{B}\right] + \nabla\cdot\mathbf{j}_{sh} \\ 
\nabla\cdot\left[\frac{1}{B^2}\nabla_\perp\left(\Phi + p_{h+}\right)\right] &=& \omega \\
\nabla\cdot{\mathbf{j}_{sh}} &=& \frac{n_e\Phi}{L_{\|}}
\end{eqnarray}

% test.tex
$\frac{\partial P}{\partial t} = -\nabla\cdot\left(P\mathbf{v}\right) - 
\frac{2}{3} P \nabla\cdot\mathbf{b}v_{\|} + 
\frac{2}{3}\nabla\cdot\left(\kappa_{\|}\mathbf{b}\mathbf{b}\cdot\nabla T\right) 
+ \frac{2}{3}S_E + S_N\frac{1}{2}mNV^2$

$E_{\|} = \left(-\nabla p_e + F\right) / n_e$

$F_z = Z n_z E_{\|}$

$\mathbf{v}_{dia} = \frac{T}{q} \nabla\times\left(\frac{\mathbf{b}}{B}\right)$

$\mathbf{v}_{pol} = - \frac{m}{q B^2} \nabla_\perp\Phi_{pol}$

\begin{eqnarray}
\frac{\partial n_n}{\partial t} &=& -\nabla\cdot\left(n_n\mathbf{b}v_{n\|} + 
n_n\mathbf{v}_{\perp n}\right) + S\\ \frac{\partial}{\partial 
t}\left(n_nv_{n\|}\right) &=& -\nabla\cdot\left(n_nv_{n\|} \mathbf{b}v_{n\|} + 
n_nv_{n\|}\mathbf{v}_{\perp n}\right) - {\bf b}\cdot{\nabla}p_n + 
\nabla_{\|}\left(D_{nn}n_n{\bf b}\cdot{\nabla}v_{n\|}\right) + F \\ \frac{\partial 
p_n}{\partial t} &=& -\nabla\cdot\left(p_n\mathbf{b}v_{n\|} + 
p_n\mathbf{v}_{\perp n}\right) - 
\frac{2}{3}p_n\nabla\cdot\left(\mathbf{b}v_{n\|}\right) + 
\nabla\cdot\left(D_{nn}n_n\nabla_\perp T_n\right) + \frac{2}{3}Q \end{eqnarray}
$\mathbf{v}_{\perp n} = -D_{nn}\frac{1}{p_n}\nabla_\perp p_n$

$c_s = \sqrt{\sum_i P_i / \sum_i m_in_i}$

\begin{eqnarray}
 \frac{\partial n_n}{\partial t} &=& \ldots + \nabla\cdot\left(\mathbf{b}D_n 
n_n{\bf b}\cdot{\nabla}p_n\right) \\ \frac{\partial p_n}{\partial t} &=& \ldots + 
\nabla\cdot\left(\mathbf{b}D_n p_n{\bf b}\cdot{\nabla}p_n\right) + 
\frac{2}{3}\nabla\cdot\left(\mathbf{b}\kappa_n {\bf b}\cdot{\nabla}T_n\right) \\ 
\frac{\partial}{\partial t}\left(n_nv_{n\|}\right) &=& \ldots + 
\nabla\cdot\left(\mathbf{b}D_n n_nv_{n\|} {\bf b}\cdot{\nabla}p_n\right) + 
\nabla\cdot\left(\mathbf{b}\eta_n {\bf b}\cdot{\nabla}T_n\right) \end{eqnarray}
$D_n = \left(\frac{B}{B_{pol}}\right)^2 \frac{T_n}{A \nu}$

$\lambda_D = \sqrt{\frac{\epsilon_0 T_e}{n_e e}}$

$\ln \lambda_{ee} = 30.4 - \frac{1}{2} \ln\left(n_e\right) + 
\frac{5}{4}\ln\left(T_e\right) - \sqrt{10^{-5} + \left(\ln T_e - 2\right)^2 / 
16}$

\begin{equation}
\ln \lambda_{ei} = \left\{\begin{array}{ll} 10 ; \textrm{if } T_e <; 0.1 
\textrm{eV or } n_e <; 10^{10}m^{-3} \\ 30 - \frac{1}{2}\ln\left(n_e\right) - 
\ln(Z) + \frac{3}{2}\ln\left(T_e\right) ; \textrm{if } T_im_e/m_i <; T_e <; 
10Z^2 \\ 31 - \frac{1}{2}\ln\left(n_e\right) + \ln\left(T_e\right) ; \textrm{if 
} T_im_e/m_i <; 10Z^2 <; T_e \\ 23 - \frac{1}{2}\ln\left(n_i\right) + 
\frac{3}{2}\ln\left(T_i\right) - \ln\left(Z^2\mu\right) ; \textrm{if } T_e <; 
T_im_e/m_i \\ \end{array}\right.\end{equation}


$\ln \lambda_{ii'} = 29.91 - ln\left[\frac{ZZ'\left(\mu + \mu'\right)}{\mu 
T_{i'} + \mu'T_i}\left(\frac{n_iZ^2}{T_i} + \frac{n_{i'} 
Z'^2}{T_{i'}}\right)^{1/2}\right]$

$\nu_{ab} = \frac{1}{3\pi^{3/2}\epsilon_0^2}\frac{Z_a^2 Z_b^2 n_b 
\ln\Lambda}{\left(v_a^2 + v_b^2\right)^{3/2}}\frac{\left(1 + m_a / 
m_b\right)}{m_a^2}$

$m_a n_a \nu_{ab} = m_b n_b \nu_{ba}$

$F_{ab} = C_m \nu_{ab} m_a n_a \left( u_b - u_a \right)$

$Q_{ab,F} = - F_{ab} u_a$

$Q_{ab,T} = \nu_{ab}\frac{3n_a m_a\left(T_b - T_a\right)}{m_a + m_b}$

$\sigma = \pi \left(\frac{d_1 + d_2}{2}\right)^2$

$v_{rel} = \sqrt{\frac{eT_1}{m_1} + \frac{eT_2}{m_2}}$

$\nu_{12} = v_{rel} n_2 \sigma$

$F_z = 0.71 n_z Z^2 \nabla_{\|}T_e$

\begin{eqnarray}
 F_z &=& \beta \nabla_{\|}T_i \\ \beta &=& \frac{3\left(\mu + 
5\sqrt{2}Z^2\left(1.1\mu^{5/2} - 0.35\mu^{3/2}\right) - 1\right)}{2.6 - 2\mu + 
5.4\mu^2} \\ \mu &=& m_z / \left(m_z + m_i\right) \end{eqnarray}
$T_{eff} = \frac{M}{M_1}T_1 + \frac{M}{M_2}T_2$

$L\left(T_e\right) = 2\times 10^{-31} \frac{\left(T_e/10\right)^3}{1 + 
\left(T_e / 10\right)^{4.5}}$

\begin{equation}
L\left(T_e\right) = \left\{\begin{array}{cl} 5.9\times 10^{-34}\frac{\sqrt{T_e 
- 1}\left(80 - T_e\right)}{1 + 3.1\times 10^{-3}\left(T_e - 1\right)^2} ; 
\textrm{If $1 <; T_e <; 80$eV} \\ 0 ; 
\textrm{Otherwise}\end{array}\right.\end{equation}


\begin{equation}
L\left(T\right) = \left\{\begin{array}{cl} \sum_{i=0}^5 a_i T_e^i ; \textrm{If 
$3 \le T_e <; 100$eV} \\ 7\times 10^{-35} \left(T_e - 2\right) + 10^{-35} ; 
\textrm{If $2 \le T_e <; 3$eV} \\ 10^{-35}\left(T_e - 1\right) ; \textrm{If $1 
<; T_e <; 2$eV} \\ 0 ; \textrm{Otherwise}\end{array}\right.\end{equation}


\begin{equation}
L\left(T\right) = \left\{\begin{array}{cl} \sum_{i=0}^9 b_i T_e^i ; \textrm{If 
$1.5 \le T_e <; 100$eV} \\ 5\times 10^{-35} \left(T_e - 1\right) ; \textrm{If 
$1 \le T_e <; 1.5$eV} \\ 0 ; \textrm{Otherwise}\end{array}\right.\end{equation}


$\nabla\cdot\left(\frac{\overline{A}\overline{n}}{B^2}\nabla_\perp \Phi + 
\sum_i\frac{A_i}{B^2}\nabla_\perp p_i\right) = \Omega$

$\nabla\cdot\left(\sum_i \frac{A_i n_i}{B^2}\nabla_\perp \Phi + \sum_i 
\frac{A_i}{B^2}\nabla_\perp p_i\right) = \Omega$

$\sum_i A_i n_i \rightarrow \overline{A}\overline{n}$

$p_s = m_s n_s v_{s\|} + Z_s e n_s A_{\|}$

$p_s = A n v_{\|} + Z n A_{\|}$

$j_{\|} = -\frac{1}{\mu_0}\nabla_\perp^2 A_{\|}$

$j_{\|} = - \frac{1}{\beta_{em}}\nabla_\perp^2 A_{\|}$

$\beta_{em} = \frac{\mu_0 e \overline{n} \overline{T}}{\overline{B}^2}$

$- \frac{1}{\beta_{em}} \nabla_\perp^2 A_{\|} + \sum_s \frac{Z^2 n_s}{A}A_{\|} 
= \sum_s \frac{Z}{A} p_s$

%components.tex
$\frac{\partial P}{\partial t} = -\nabla\cdot\left(P\mathbf{v}\right) - 
\frac{2}{3} P \nabla\cdot\mathbf{b}v_{\|} + 
\frac{2}{3}\nabla\cdot\left(\kappa_{\|}\mathbf{b}\mathbf{b}\cdot\nabla T\right) 
+ \frac{2}{3}S_E + S_N\frac{1}{2}mNV^2$

$E_{\|} = \left(-\nabla p_e + F\right) / n_e$

$F_z = Z n_z E_{\|}$

$\mathbf{v}_{dia} = \frac{T}{q} \nabla\times\left(\frac{\mathbf{b}}{B}\right)$

$\mathbf{v}_{pol} = - \frac{m}{q B^2} \nabla_\perp\Phi_{pol}$

\begin{eqnarray}
\frac{\partial n_n}{\partial t} &=& -\nabla\cdot\left(n_n\mathbf{b}v_{n\|} + 
n_n\mathbf{v}_{\perp n}\right) + S\\ \frac{\partial}{\partial 
t}\left(n_nv_{n\|}\right) &=& -\nabla\cdot\left(n_nv_{n\|} \mathbf{b}v_{n\|} + 
n_nv_{n\|}\mathbf{v}_{\perp n}\right) - {\bf b}\cdot{\nabla}p_n + 
\nabla_{\|}\left(D_{nn}n_n{\bf b}\cdot{\nabla}v_{n\|}\right) + F \\ \frac{\partial 
p_n}{\partial t} &=& -\nabla\cdot\left(p_n\mathbf{b}v_{n\|} + 
p_n\mathbf{v}_{\perp n}\right) - 
\frac{2}{3}p_n\nabla\cdot\left(\mathbf{b}v_{n\|}\right) + 
\nabla\cdot\left(D_{nn}n_n\nabla_\perp T_n\right) + \frac{2}{3}Q \end{eqnarray}
$\mathbf{v}_{\perp n} = -D_{nn}\frac{1}{p_n}\nabla_\perp p_n$

$c_s = \sqrt{\sum_i P_i / \sum_i m_in_i}$

\begin{eqnarray}
 \frac{\partial n_n}{\partial t} &=& \ldots + \nabla\cdot\left(\mathbf{b}D_n 
n_n{\bf b}\cdot{\nabla}p_n\right) \\ \frac{\partial p_n}{\partial t} &=& \ldots + 
\nabla\cdot\left(\mathbf{b}D_n p_n{\bf b}\cdot{\nabla}p_n\right) + 
\frac{2}{3}\nabla\cdot\left(\mathbf{b}\kappa_n {\bf b}\cdot{\nabla}T_n\right) \\ 
\frac{\partial}{\partial t}\left(n_nv_{n\|}\right) &=& \ldots + 
\nabla\cdot\left(\mathbf{b}D_n n_nv_{n\|} {\bf b}\cdot{\nabla}p_n\right) + 
\nabla\cdot\left(\mathbf{b}\eta_n {\bf b}\cdot{\nabla}T_n\right) \end{eqnarray}
$D_n = \left(\frac{B}{B_{pol}}\right)^2 \frac{T_n}{A \nu}$

$\lambda_D = \sqrt{\frac{\epsilon_0 T_e}{n_e e}}$

$\ln \lambda_{ee} = 30.4 - \frac{1}{2} \ln\left(n_e\right) + 
\frac{5}{4}\ln\left(T_e\right) - \sqrt{10^{-5} + \left(\ln T_e - 2\right)^2 / 
16}$

\begin{equation}
\ln \lambda_{ei} = \left\{\begin{array}{ll} 10 ; \textrm{if } T_e <; 0.1 
\textrm{eV or } n_e <; 10^{10}m^{-3} \\ 30 - \frac{1}{2}\ln\left(n_e\right) - 
\ln(Z) + \frac{3}{2}\ln\left(T_e\right) ; \textrm{if } T_im_e/m_i <; T_e <; 
10Z^2 \\ 31 - \frac{1}{2}\ln\left(n_e\right) + \ln\left(T_e\right) ; \textrm{if 
} T_im_e/m_i <; 10Z^2 <; T_e \\ 23 - \frac{1}{2}\ln\left(n_i\right) + 
\frac{3}{2}\ln\left(T_i\right) - \ln\left(Z^2\mu\right) ; \textrm{if } T_e <; 
T_im_e/m_i \\ \end{array}\right.\end{equation}


$\ln \lambda_{ii'} = 29.91 - ln\left[\frac{ZZ'\left(\mu + \mu'\right)}{\mu 
T_{i'} + \mu'T_i}\left(\frac{n_iZ^2}{T_i} + \frac{n_{i'} 
Z'^2}{T_{i'}}\right)^{1/2}\right]$

$\nu_{ab} = \frac{1}{3\pi^{3/2}\epsilon_0^2}\frac{Z_a^2 Z_b^2 n_b 
\ln\Lambda}{\left(v_a^2 + v_b^2\right)^{3/2}}\frac{\left(1 + m_a / 
m_b\right)}{m_a^2}$

$m_a n_a \nu_{ab} = m_b n_b \nu_{ba}$

$F_{ab} = C_m \nu_{ab} m_a n_a \left( u_b - u_a \right)$

$Q_{ab,F} = - F_{ab} u_a$

$Q_{ab,T} = \nu_{ab}\frac{3n_a m_a\left(T_b - T_a\right)}{m_a + m_b}$

$\sigma = \pi \left(\frac{d_1 + d_2}{2}\right)^2$

$v_{rel} = \sqrt{\frac{eT_1}{m_1} + \frac{eT_2}{m_2}}$

$\nu_{12} = v_{rel} n_2 \sigma$

$F_z = 0.71 n_z Z^2 \nabla_{\|}T_e$

\begin{eqnarray}
 F_z &=& \beta \nabla_{\|}T_i \\ \beta &=& \frac{3\left(\mu + 
5\sqrt{2}Z^2\left(1.1\mu^{5/2} - 0.35\mu^{3/2}\right) - 1\right)}{2.6 - 2\mu + 
5.4\mu^2} \\ \mu &=& m_z / \left(m_z + m_i\right) \end{eqnarray}
$T_{eff} = \frac{M}{M_1}T_1 + \frac{M}{M_2}T_2$

$L\left(T_e\right) = 2\times 10^{-31} \frac{\left(T_e/10\right)^3}{1 + 
\left(T_e / 10\right)^{4.5}}$

\begin{equation}
L\left(T_e\right) = \left\{\begin{array}{cl} 5.9\times 10^{-34}\frac{\sqrt{T_e 
- 1}\left(80 - T_e\right)}{1 + 3.1\times 10^{-3}\left(T_e - 1\right)^2} ; 
\textrm{If $1 <; T_e <; 80$eV} \\ 0 ; 
\textrm{Otherwise}\end{array}\right.\end{equation}


\begin{equation}
L\left(T\right) = \left\{\begin{array}{cl} \sum_{i=0}^5 a_i T_e^i ; \textrm{If 
$3 \le T_e <; 100$eV} \\ 7\times 10^{-35} \left(T_e - 2\right) + 10^{-35} ; 
\textrm{If $2 \le T_e <; 3$eV} \\ 10^{-35}\left(T_e - 1\right) ; \textrm{If $1 
<; T_e <; 2$eV} \\ 0 ; \textrm{Otherwise}\end{array}\right.\end{equation}


\begin{equation}
L\left(T\right) = \left\{\begin{array}{cl} \sum_{i=0}^9 b_i T_e^i ; \textrm{If 
$1.5 \le T_e <; 100$eV} \\ 5\times 10^{-35} \left(T_e - 1\right) ; \textrm{If 
$1 \le T_e <; 1.5$eV} \\ 0 ; \textrm{Otherwise}\end{array}\right.\end{equation}


$\nabla\cdot\left(\frac{\overline{A}\overline{n}}{B^2}\nabla_\perp \Phi + 
\sum_i\frac{A_i}{B^2}\nabla_\perp p_i\right) = \Omega$

$\nabla\cdot\left(\sum_i \frac{A_i n_i}{B^2}\nabla_\perp \Phi + \sum_i 
\frac{A_i}{B^2}\nabla_\perp p_i\right) = \Omega$

$\sum_i A_i n_i \rightarrow \overline{A}\overline{n}$

$p_s = m_s n_s v_{s\|} + Z_s e n_s A_{\|}$

$p_s = A n v_{\|} + Z n A_{\|}$

$j_{\|} = -\frac{1}{\mu_0}\nabla_\perp^2 A_{\|}$

$j_{\|} = - \frac{1}{\beta_{em}}\nabla_\perp^2 A_{\|}$

$\beta_{em} = \frac{\mu_0 e \overline{n} \overline{T}}{\overline{B}^2}$

$- \frac{1}{\beta_{em}} \nabla_\perp^2 A_{\|} + \sum_s \frac{Z^2 n_s}{A}A_{\|} 
= \sum_s \frac{Z}{A} p_s$

